---
title: "18: Linear Operators"
author: "Derek Sollberger"
date: "2023-03-06"
# format: 
#   revealjs:
#     scrollable: true
format: html
# server: shiny
---

\newcommand{\ds}{\displaystyle}

```{r}
#| echo: false
#| message: false
#| warning: false
library("tidyverse")
```

:::{.callout-tip}
## Previously, in Math 32,

- $X$ is a random variable with PDF $f$
- $Y$ is a random variable with PDF $g$


$${\color{blue}\text{E}[X] = \ds\int_{-\infty}^{\infty} \! x \cdot f(x) \, dx}, \quad {\color{red}\text{E}[Y] = \ds\int_{-\infty}^{\infty} \! y \cdot g(y) \, dy}$$

$${\color{blue}\text{Var}(X) = \text{E}[X^{2}] - \left( \text{E}[X] \right)^{2}}, \quad {\color{red}\text{Var}(Y) = \text{E}[Y^{2}] - \left( \text{E}[Y] \right)^{2}}$$

Let $a$, $b$, and $c$ be constants.
:::


## Linear Operators

:::{.callout-note}
## Linear Operators

We say that $L$ is a **linear operator** if 

$$\begin{array}{rcl}
  L(a{\color{blue}f(x)}) & = & aL({\color{blue}f(x)}) \\
  L({\color{blue}f(x)} + {\color{red}g(x)}) & = & L({\color{blue}f(x)}) + L({\color{red}g(x)}) \\
\end{array}$$
:::

:::{.callout-tip}
## Linear Operators

Loosely translated, $L$ is a linear operator if

- we can factor out a scalar multiple
- we can split the operator across a sum or difference
:::


## Calculus Review

:::: {.columns}

::: {.column width="50%"}
- Show that the derivative operator is a linear operator.	
- Show that the integral operator is a linear operator.
:::

::: {.column width="50%"}
![](derivativepun.png)
:::

::::

:::{.callout-tip collapse="true"}
## Claim: the derivative operator is a linear operator

**Proof**

\begin{array}{rcl}
      \ds\frac{d}{dx}(a{\color{blue}f(x)} + b{\color{red}g(x)}) & = & \ds\frac{d}{dx} a{\color{blue}f(x)} + \ds\frac{d}{dx} b{\color{red}g(x)} \\
      ~ & = &  a\ds\frac{d}{dx} {\color{blue}f(x)} + b\ds\frac{d}{dx} {\color{red}g(x)} \\
    \end{array}
    
$$\ds\frac{d}{dx}(a{\color{blue}f(x)} + b{\color{red}g(x)}) = a\ds\frac{d}{dx} {\color{blue}f(x)} + b\ds\frac{d}{dx} {\color{red}g(x)},$$

so $\ds\frac{d}{dx}$ is a linear operator.
:::

:::{.callout-tip collapse="true"}
## Claim: the integral operator is a linear operator

**Proof**

\begin{array}{rcl}
      \ds\int \! (a{\color{blue}f(x)} + b{\color{red}g(x)}) \, dx & = & \ds\int \! a{\color{blue}f(x)} \, dx + \ds\int \! b{\color{red}g(x)} \, dx \\
      ~ & = & a\ds\int \! {\color{blue}f(x)} \, dx + b\ds\int \! {\color{red}g(x)} \, dx \\
    \end{array}
    
$$\ds\int \! (a{\color{blue}f(x)} + b{\color{red}g(x)}) \, dx = a\ds\int \! {\color{blue}f(x)} \, dx + b\ds\int \! {\color{red}g(x)} \, dx,$$

so $\ds\int$ is a linear operator. 
:::


## Expected Value

Is the expectation operator $\text{E}$ a linear operator?

:::{.callout-tip collapse="true"}
## Claim: $\text{E}[aX] = a\text{E}[X]$

**Proof**

$$\text{E}[aX] = \ds\int_{-\infty}^{\infty} \! ax \cdot f(x) \, dx = a{\color{blue}\ds\int_{-\infty}^{\infty} \! x \cdot f(x) \, dx} = a{\color{blue}\text{E}[X]}$$
        
We have shown that we can factor out a scalar multiple across the expectation operator.
:::


:::{.callout-tip collapse="true"}
## Claim: $\text{E}[X + c] = \text{E}[X] + c$

**Proof**

\begin{array}{rcl}
          \text{E}[X + c] & = & \ds\int_{-\infty}^{\infty} \! (x + c) \cdot f(x) \, dx \\
          ~ & = & {\color{blue}\ds\int_{-\infty}^{\infty} \! x \cdot f(x) \, dx} + \ds\int_{-\infty}^{\infty} \! c \cdot f(x) \, dx\\
          ~ & = & {\color{blue}\ds\int_{-\infty}^{\infty} \! x \cdot f(x) \, dx} + c\ds\int_{-\infty}^{\infty} \! f(x) \, dx \\
          ~ & = & {\color{blue}\text{E}[X]} + c \\
        \end{array}
        
We have shown that a horizontal shift of $c$ units in the data also affects the expected value by $c$ units
:::

:::{.callout-tip collapse="true"}
## Claim: $\text{E}[X + Y] = \text{E}[X] + \text{E}[Y]$

**Proof**

\begin{array}{rcl}
          {\color{purple}\text{E}[X + Y]} & = & {\color{blue}\ds\int_{-\infty}^{\infty}}{\color{red}\ds\int_{-\infty}^{\infty}} \! {\color{purple}(x + y) \cdot f(x,y)} \, {\color{red}dy} \, {\color{blue}dx} \\
          ~ & = & {\color{blue}\ds\int_{-\infty}^{\infty}}{\color{red}\ds\int_{-\infty}^{\infty}} \! {\color{blue}x} \cdot {\color{purple}f(x,y)} \, {\color{red}dy} \, {\color{blue}dx}  + {\color{red}\ds\int_{-\infty}^{\infty}}{\color{blue}\ds\int_{-\infty}^{\infty}} \! {\color{red}y} \cdot {\color{purple}f(x,y)} \, {\color{blue}dx} \, {\color{red}dy} \\
          ~ & = & {\color{blue}\ds\int_{-\infty}^{\infty}\! x \cdot f_{X}(x) \, dx}  + {\color{red}\ds\int_{-\infty}^{\infty} \! y \cdot f_{Y}(y) \, dy} \\
          ~ & = & {\color{blue}\text{E}[X]} + {\color{red}\text{E}[Y]} \\
        \end{array}
        
We have shown that the expected value of a sum \\ is the sum of the expected values.
:::


:::{.callout-tip collapse="true"}
## Conclusion

Combining the above results, since

$$\text{E}[aX + bY] = a\text{E}[X] + b\text{E}[Y]$$

we have shown that the expectation operator $\text{E}$ is a linear operator.
        
Also,
        
$$\text{E}[aX + bY + c] = a\text{E}[X] + b\text{E}[Y] + c$$
:::


## Variance

Is the variance $\text{Var}(X)$ function a linear operator?

:::{.callout-tip collapse="true"}
## Claim: $\text{Var}(aX) = a\text{Var}(X)$

**Counterpoint:**  

Recall the ``practical formula for variance'' 

$$\text{Var}(X) = \text{E}[X^{2}] - \left(\text{E}[X]\right)^{2}$$

and tracking the scaling factor proceeds as follows

\begin{array}{rcl}
          \text{Var}(aX) & = & \text{E}[(aX)^{2}] - \left(\text{E}[aX]\right)^{2} \\
          ~ & = & \ds\int_{-\infty}^{\infty}\! (ax)^{2} \cdot f(x) \, dx - \left(a\text{E}[X]\right)^{2} \\
          ~ & = & \ds\int_{-\infty}^{\infty}\! a^{2}x^{2} \cdot f(x) \, dx - a^{2}\left(\text{E}[X]\right)^{2} \\
          ~ & = & a^{2} \left[ \ds\int_{-\infty}^{\infty}\! x^{2} \cdot f(x) \, dx - \left(\text{E}[X]\right)^{2} \right] \\
          ~ & = & a^{2} \left( \text{E}[X^{2}] - \left(\text{E}[X]\right)^{2} \right) \\
          ~ & = & a^{2} \text{Var}(X) \\
        \end{array}
        
When factoring out a scalar from the variance function, *the factor is squared*.

Furthermore, since $\text{Var}(aX) \neq a\text{Var}(X)$, we have shown that the variance function is *not* a linear operator.
:::

:::{.callout-tip collapse="true"}
## Claim: $\text{Var}(X + c) = \text{Var}(X) + c$

**Counterpoint:**  

Recall the ``practical formula for variance'' 
        
\begin{array}{rcl}
          \text{Var}(X + c) & = & \text{E}[(X + c)^{2}] - \left(\text{E}[X + c]\right)^{2} \\
          ~ & = & \text{E}[X^{2} + 2cX + c^{2}] - \left(\text{E}[X] + c \right)^{2} \\
          ~ & = & \text{E}[X^{2}] + \text{E}[2cX] + \text{E}[c^{2}] - \left(\text{E}[X]\right)^{2} - 2c\text{E}[X] - c^{2} \\
          ~ & = & \text{E}[X^{2}] + 2c\text{E}[X] + c^{2} - \left(\text{E}[X]\right)^{2} - 2c\text{E}[X] - c^{2} \\
          ~ & = & \text{E}[X^{2}] - \left(\text{E}[X]\right)^{2} \\
          ~ & = & \text{Var}(X) \\
        \end{array}
        
We have shown that $\text{Var}(X + c) = \text{Var}(X)$.  That is, variance is not affected by a horizontal shift (phase shift)!


Furthermore, since $\text{Var}(X + c) \neq \text{Var}(X) + c$, we have shown that the variance function is not a linear operator.
:::


:::{.callout-tip collapse="true"}
## Claim: $\text{Var}(X + Y) = {\color{blue}\text{Var}(X)} + {\color{red}\text{Var}(Y)}$

**Counterpoint:**  

\begin{array}{rcl}
          \text{Var}(X + Y) & = & \text{E}[(X + Y)^{2}] - \left(\text{E}[X + Y]\right)^{2} \\
          ~ & = & \text{E}[X^{2} + 2XY + Y^{2}] - \left(\text{E}[X] + \text{E}[Y]\right)^{2} \\
          ~ & = & \text{E}[X^{2}] + \text{E}[2XY] + \text{E}[Y^{2}] - \left(\text{E}[X]\right)^{2}+ 2\text{E}[X]\text{E}[Y] + \left(\text{E}[Y]\right)^{2} \\
          ~ & = & \text{E}[X^{2}] - \left(\text{E}[X]\right)^{2}  + \text{E}[Y^{2}] - \left(\text{E}[Y]\right)^{2} + 2\text{E}[XY] - 2\text{E}[X]\text{E}[Y] \\
          ~ & = & {\color{blue}\text{Var}(X)} + {\color{red}\text{Var}(Y)} + 2\left( {\color{purple}\text{E}[XY] - \text{E}[X]\text{E}[Y] } \right) \\
        \end{array}
    
We have shown that $\text{Var}(X + Y) \neq \text{Var}(X) + \text{Var}(Y)$.  That is, the variance of the sum is not the sum of the variances (unless ...?)

Furthermore, since $\text{Var}(X + Y) \neq \text{Var}(X) + \text{Var}(Y)$, we have shown that the variance function is not a linear operator.
:::

:::{.callout-warning collapse="true"}
## Conclusion

We have shown that the variance function is not a linear operator.
        
Next time: working with 

$${\color{purple}\text{E}[XY] - \text{E}[X]\text{E}[Y]}$$

which is called the **covariance**!
:::


## Looking Ahead

:::: {.columns}

::: {.column width="60%"}
- due Fri., Mar. 10:
  - WHW7
  - LHW6
  - Internet Connection (survey)
  
- Exam 2 will be on Mon., Apr. 10

- no lecture on Mar. 10, Mar. 24

:::

::: {.column width="40%"}
![](logic.png)

[tweet source](https://mobile.twitter.com/CMastication/status/1582548812987772929)
:::

::::

















:::: {.columns}

::: {.column width="50%"}
	
:::

::: {.column width="50%"}

:::

::::

::::: {.panel-tabset}



:::::
